Rename circuit_increase_input_count

src/compiler.ml
@@ -302,7 +302,7 @@ let circuit_let_data (type a) (env : Environ.env) (f : (int -> circuit) -> circu
 let circuit_let (env : Environ.env) (f : (int -> circuit) -> circuit) (c : circuit) : circuit =
   circuit_let_data env (fun c -> (f c, ())) c |> fst
 
-let circuit_grow_input_count (env : Environ.env) (c : circuit) (additional_input_count : int) : circuit =
+let circuit_increase_input_count (env : Environ.env) (c : circuit) (additional_input_count : int) : circuit =
   {
     circuit_input_count = c.circuit_input_count + additional_input_count;
     circuit_wire_count = c.circuit_wire_count;
@@ -310,7 +310,7 @@ let circuit_grow_input_count (env : Environ.env) (c : circuit) (additional_input
     circuit_output_wires = c.circuit_output_wires;
     circuit_with_wf_and_spec_constr =
       EConstr.mkApp (
-        get_ref env "vcpu.circuit.grow_input_count_with_wf_and_spec",
+        get_ref env "vcpu.circuit.increase_input_count_with_wf_and_spec",
         [|
           EConstr.mkApp (
             get_ref env "vcpu.circuit_with_wf_and_spec.circuit_with_wf",
